use macros instead of elaboration for embeddings

Lott/Data/Option.lean
@@ -1,5 +1,18 @@
 namespace Option
 
+def someIf (x : α) (b : Bool) : Option α := if b then some x else none
+
+theorem someIf_true : someIf x true = some x := rfl
+
+theorem eq_of_someIf_eq_some : someIf x b = some y → x = y ∧ b = true := by
+  intro eq
+  rw [someIf] at eq
+  split at eq
+  · case isTrue h => exact ⟨some.inj eq, h⟩
+  · case isFalse => nomatch eq
+
+def keepIf (x : Option α) (b : Bool) : Option α := if b then x else none
+
 def mapMem (a? : Option α) (f : (a : α) → a ∈ a? → β) : Option β := match a? with
   | some a => f a rfl
   | none => none
