Lott/Elab/Basic.lean
@@ -10,7 +10,7 @@ import Lott.IR
 -- TODO: Test stuff without locally nameless.
 -- TODO: Centralize validation of bind/id usage in nonterminals.
 
-namespace Lott.Elab
+namespace Lott
 
 open Lean
 open Lean.Elab
@@ -23,61 +23,9 @@ open Lean.Parser.Syntax
 open Lean.Parser.Term
 open Lott.IR
 
-/- Term embedding syntax. -/
-
-abbrev TermElab := Bool → Syntax → TermElabM Expr
-
-private unsafe
-def mkLottTermElabAttributeUnsafe (ref : Name) : IO (KeyedDeclsAttribute TermElab) := do
-  mkElabAttribute TermElab .anonymous `lott_term_elab `Lott `Lott.Elab.TermElab "lott" ref
-
-@[implemented_by mkLottTermElabAttributeUnsafe]
-opaque mkLottTermElabAttribute (ref : Name) : IO (KeyedDeclsAttribute TermElab)
-
-initialize lottTermElabAttribute : KeyedDeclsAttribute TermElab ← mkLottTermElabAttribute decl_name%
-
-partial
-def elabTerm (catName : Name) : TermElab := fun isBinder stx => do
-  let result ← liftMacroM <| expandMacroImpl? (← getEnv) stx
-  match result with
-  | some (decl, stxNew?) => do
-    let stxNew ← liftMacroM <| liftExcept stxNew?
-    withInfoContext' stx (mkInfo := mkTermInfo decl stx)
-      (mkInfoOnError := mkPartialTermInfo decl stx) <|
-      withMacroExpansion stx stxNew <|
-        withRef stxNew <|
-          elabTerm catName isBinder stxNew
-  | none => match lottTermElabAttribute.getEntries (← getEnv) catName with
-    | [] =>
-      throwError "term elaboration function for '{catName}' has not been implemented{indentD stx}"
-    | elabFns => elabTermWithFns isBinder stx elabFns
-where
-  elabTermWithFns isBinder stx
-    | [] => unreachable!
-    | [elabFn] => elabFn.value isBinder stx
-    | elabFn :: elabFns => do
-      try
-        elabFn.value false stx
-      catch ex => match ex with
-        | .internal id _ =>
-          if id == unsupportedSyntaxExceptionId then
-            elabTermWithFns isBinder stx elabFns
-          else
-            throw ex
-        | _ => throw ex
-
-@[term_elab lott_symbol_embed]
-private
-def symbolEmbedElab : Term.TermElab := fun stx _ => do
-  let stx := stx[3]!
-  elabTerm stx.getKind false stx
-
-elab_rules : term
-  | `([[$stx:Lott.Symbol]]) => elabTerm stx.raw.getKind false stx
-  | `([[$stx:Lott.Judgement]]) => elabTerm stx.raw.getKind false stx
-
 /- Utility stuff. -/
 
+private
 def resolveSymbol (symbolName : Ident) (allowSuffix := true) : CommandElabM Name := do
   let name := symbolName.getId
   let state := aliasExt.getState (← getEnv)
@@ -149,20 +97,9 @@ def _root_.Lott.IR.ofStx (stx : TSyntax `stx) (l? : Option Ident := none) : Comm
   | _ => throwUnsupportedSyntax
 
 partial
-def _root_.Lott.IR.ofProdArg (arg : TSyntax `Lott.prodArg) : CommandElabM IR := do
+def _root_.Lott.IR.ofProdArg (arg : TSyntax ``Lott.prodArg) : CommandElabM IR := do
   let `(prodArg| $[$l?:ident:]?$stx:stx) := arg | throwUnsupportedSyntax
   ofStx stx l?
-
-private
-def mkMkProd (entries : Array (Term × Term)) : CommandElabM (Option (Term × Term)) := do
-  let some back := entries.back? | return none
-  let res ← entries.foldrM (start := entries.size - 1) (init := back)
-    fun (expr, type) (mkProdAcc, typeAcc) =>
-    return (
-      ← ``(mkApp4 (Expr.const `Prod.mk [0, 0]) $type $typeAcc $expr $mkProdAcc),
-      ← ``(mkApp2 (Expr.const `Prod [0, 0]) $type $typeAcc)
-    )
-  return some res
 
 private partial
 def _root_.Lott.IR.toExprArgs (ir : Array IR) (ids binders : Array Name)
@@ -173,98 +110,108 @@ def _root_.Lott.IR.toExprArgs (ir : Array IR) (ids binders : Array Name)
 
       return some l
 
-private
-def elabListComprehension (symbol : TSyntax `Lott.Symbol) (pat : Term) (collection : Term)
-  (type : Expr) : TermElabM Expr := do
-  let stx ← `($collection |>.map (fun $pat => [[$symbol:Lott.Symbol]]) |>.flatten)
-  Term.elabTerm stx <| Expr.app (.const `List [levelOne]) type
+def Syntax.mkSymbolEmbed (stx : Syntax) : Term :=
+  .mk <| mkNode ``Lott.symbolEmbed #[mkAtom "[[", stx, mkAtom "]]"]
 
-private
-def elabOptionComprehension (symbol : TSyntax `Lott.Symbol) (condition : Term) (type : Expr)
-  : TermElabM Expr := do
-  let stx ← `([[$symbol:Lott.Symbol]].filter fun _ => $condition)
-  Term.elabTerm stx <| Expr.app (.const `Option [levelOne]) type
+def _root_.Lean.Syntax.mkTypeAscription (stx type : Syntax) : Term :=
+  .mk <| mkNode ``Lean.Parser.Term.typeAscription
+    #[mkAtom "(", stx, mkAtom ":", mkNullNode #[type], mkAtom ")"]
+
+def _root_.Lean.Syntax.mkMap (collection pat body : Term) (mapName : Name) : MacroM Term :=
+  `($(collection).$(mkIdent mapName):ident fun $pat => $body)
 
 private partial
 def _root_.Lott.IR.toTermSeqItems (ir : Array IR) (canon : Name) (ids binders : Array Name)
-  : CommandElabM (TSyntaxArray `Lean.Parser.Term.doSeqItem) :=
+  : CommandElabM (TSyntaxArray ``Lean.Parser.Term.doSeqItem) :=
   ir.filterMapM fun
-    | mk l (.category n) => do
+    | mk l (.category _) => do
       if binders.contains l.getId then
         return none
 
-      `(doSeqItem|
-          let $l ← Lott.Elab.elabTerm $(quote <| symbolPrefix ++ n)
-            $(quote <| ids.contains l.getId) $l)
+      `(doSeqItem| let $l := Lott.Syntax.mkSymbolEmbed $l)
     | mk _ (.atom _) => return none
     | mk l (.sepBy ir sep) => do
       let catName := sepByPrefix ++ (← getCurrNamespace) ++ canon ++ l.getId |>.obfuscateMacroScopes
       let patternArgs ← IR.toPatternArgs ir
       let seqItems ← IR.toTermSeqItems ir canon ids binders
       let exprArgs ← IR.toExprArgs ir ids binders
-      let exprTypes ← ir.filterMapM <| IR.toMkTypeExpr ids binders
-      let some (mkProd, type) ← mkMkProd (exprArgs.getElems.zip exprTypes) | return none
-
-      let termElabIdent := mkIdentFrom l <| canon ++ l.getId.appendAfter "TermElab"
-      elabCommand <| ←
-        `(@[lott_term_elab $(mkIdent catName)] def $termElabIdent : Lott.Elab.TermElab
-            | _, Syntax.node _ $(quote catName) #[
-              Lean.Syntax.atom _ "</",
-              symbol,
-              Lean.Syntax.atom _ "//",
-              pat,
-              Lean.Syntax.atom _ "in",
-              collection,
-              Lean.Syntax.atom _ "/>"
-            ] => do
-              elabListComprehension (TSyntax.mk symbol) (TSyntax.mk pat) (TSyntax.mk collection) $type
-            | _, Syntax.node _ $(quote catName) #[
-                lhs@(Syntax.node _ $(quote catName) _),
-                Lean.Syntax.atom _ $(quote sep.trim),
-                rhs@(Syntax.node _ $(quote catName) _)
-              ] => do
-              let lhs ← Lott.Elab.elabTerm $(quote catName) false lhs
-              let rhs ← Lott.Elab.elabTerm $(quote catName) false rhs
-              Meta.liftMetaM <| Meta.reduceAll <| mkApp3 (Expr.const `List.append [0]) $type lhs rhs
-            | _, Syntax.node _ $(quote catName) #[$patternArgs,*] => do
-              $seqItems*
-              return mkApp3 (Expr.const `List.cons [0]) $type $mkProd <| Expr.app (Expr.const `List.nil [0]) $type
-            | _, _ => no_error_if_unused% Lean.Elab.throwUnsupportedSyntax)
+      let go ← mkFreshIdent l
 
       `(doSeqItem| let $l ← match (Syntax.getArgs $l)[0]? with
-          | some stx => Lott.Elab.elabTerm $(quote catName) false stx
-          | none => pure <| Expr.app (Expr.const `List.nil [0]) $type)
+          | some stx =>
+            let rec $go:ident : Lean.Syntax → Lean.MacroM (Bool × Lean.Syntax.Term)
+              | Lean.Syntax.node _ $(quote catName) #[
+                  Lean.Syntax.atom _ "</",
+                  symbol,
+                  Lean.Syntax.atom _ "//",
+                  pat,
+                  Lean.Syntax.atom _ "in",
+                  collection,
+                  Lean.Syntax.atom _ "/>"
+                ] => do
+                let (singleton, symbol) ← $go:ident symbol
+                let mapName := if singleton then `map else `flatMap
+                return (false, ← Lean.Syntax.mkMap (.mk collection) (.mk pat) (.mk symbol) mapName)
+              | Lean.Syntax.node _ $(quote catName) #[
+                  lhs@(Lean.Syntax.node _ $(quote catName) _),
+                  Lean.Syntax.atom _ $(quote sep.trim),
+                  rhs@(Lean.Syntax.node _ $(quote catName) _)
+                ] => do
+                let (lhsSingleton, lhs) ← $go:ident lhs
+                let (rhsSingleton, rhs) ← $go:ident rhs
+                let combineName := if lhsSingleton then ``List.cons else ``HAppend.hAppend
+                let rhs := if rhsSingleton then
+                    Lean.Syntax.mkCApp ``List.cons #[rhs, Lean.mkIdent ``List.nil]
+                  else
+                    rhs
+                return (false, Lean.Syntax.mkCApp combineName #[lhs, rhs])
+              | Lean.Syntax.node _ $(quote catName) #[$patternArgs,*] => do
+                $seqItems*
+                return (true, ← Lott.IR.foldrProd #[$exprArgs,*])
+              | _ => Lean.Macro.throwUnsupported
+            let (singleton, x) ← $go:ident stx
+            if singleton then
+              pure <| Lean.Syntax.mkCApp ``List.cons #[x, Lean.mkIdent ``List.nil]
+            else
+              pure x
+          | none => pure <| mkIdent ``List.nil)
     | mk l (.optional ir) => do
       let catName := sepByPrefix ++ (← getCurrNamespace) ++ canon ++ l.getId |>.obfuscateMacroScopes
       let patternArgs ← IR.toPatternArgs ir
       let seqItems ← IR.toTermSeqItems ir canon ids binders
       let exprArgs ← IR.toExprArgs ir ids binders
-      let exprTypes ← ir.filterMapM <| IR.toMkTypeExpr ids binders
-      let some (mkProd, type) ← mkMkProd (exprArgs.getElems.zip exprTypes) | return none
-
-      let termElabIdent := mkIdentFrom l <| canon ++ l.getId.appendAfter "TermElab"
-      elabCommand <| ←
-        `(@[lott_term_elab $(mkIdent catName)] def $termElabIdent : Lott.Elab.TermElab
-            | _, Syntax.node _ $(quote catName) #[
-              Lean.Syntax.atom _ "</",
-              symbol,
-              Lean.Syntax.atom _ "//",
-              condition,
-              Lean.Syntax.atom _ "/>"
-            ] => do
-              elabOptionComprehension (TSyntax.mk symbol) (TSyntax.mk condition) $type
-            | _, Syntax.node _ $(quote catName) #[$patternArgs,*] => do
-              $seqItems*
-              return mkApp2 (Expr.const `Option.some [0]) $type $mkProd
-            | _, _ => no_error_if_unused% Lean.Elab.throwUnsupportedSyntax)
+      let go ← mkFreshIdent l
 
       `(doSeqItem| let $l ← match (Syntax.getArgs $l)[0]? with
-          | some stx => Lott.Elab.elabTerm $(quote catName) false stx
-          | none => pure <| Expr.app (Expr.const `Option.none [0]) $type)
+          | some stx =>
+            let rec $go:ident : Lean.Syntax → Lean.MacroM (Bool × Lean.Syntax.Term)
+              | Lean.Syntax.node _ $(quote catName) #[
+                  Lean.Syntax.atom _ "</",
+                  symbol,
+                  Lean.Syntax.atom _ "//",
+                  cond,
+                  Lean.Syntax.atom _ "/>"
+                ] => do
+                let (option, symbol) ← $go:ident symbol
+                let modifierName := if option then ``Option.keepIf else ``Option.someIf
+                return (
+                  true,
+                  Lean.Syntax.mkCApp modifierName #[symbol, .mk cond]
+                )
+              | Lean.Syntax.node _ $(quote catName) #[$patternArgs,*] => do
+                $seqItems*
+                return (false, ← Lott.IR.foldrProd #[$exprArgs,*])
+              | _ => Lean.Macro.throwUnsupported
+            let (option, x) ← $go:ident stx
+            if option then
+              pure x
+            else
+              pure <| Lean.Syntax.mkCApp ``Option.some #[x]
+          | none => pure <| mkIdent ``Option.none)
 
-partial
+private partial
 def _root_.Lott.IR.toIsChildCtor (prodIdent isIdent : Ident) (qualified pqualified : Name) (ir pir : Array IR)
-  (binders : Array Name) : CommandElabM (TSyntax `Lean.Parser.Command.ctor) := do
+  (binders : Array Name) : CommandElabM (TSyntax ``Lean.Parser.Command.ctor) := do
   if ir.size != pir.size then
     throwErrorAt prodIdent "length of child production ({ir.size}) doesn't match length of parent production ({pir.size})"
 
@@ -276,9 +223,9 @@ def _root_.Lott.IR.toIsChildCtor (prodIdent isIdent : Ident) (qualified pqualifi
   let ctorType ← foldrArrow ctorTypeArgs <| ← ``($isIdent ($(mkIdent <| pqualified ++ prodIdent.getId) $(← toTerms ctorTypeRetArgs)*))
   return ← `(ctor| | $prodIdent:ident $binders:bracketedBinder* : $ctorType)
 where
-  go (irs : Array (IR × IR)) (patAcc : TSyntaxArray `Lean.binderIdent := #[])
+  go (irs : Array (IR × IR)) (patAcc : TSyntaxArray ``Lean.binderIdent := #[])
     (propAcc : Array Term := #[])
-    : CommandElabM (TSyntaxArray `Lean.binderIdent × Array Term) := do
+    : CommandElabM (TSyntaxArray ``Lean.binderIdent × Array Term) := do
     let some (mk l' ir, mk l pir) := irs[0]? | return (patAcc, propAcc)
     let irs' := irs.extract 1 irs.size
 
@@ -294,7 +241,7 @@ where
       if n == np then
         return ← go irs' (patAcc.push hole) propAcc
 
-      if some np == ((childExt.getState (← getEnv)).find? n).map (·.parent') then
+      if some np == ((childExt.getState (← getEnv)).find? n).map (·.parent) then
         let .str _ nStr := n | throwUnsupportedSyntax
         let isName := np ++ Name.str .anonymous nStr |>.appendBefore "Is"
         return ← go irs' (patAcc.push lbi) <| propAcc.push <| ← `($(mkIdent isName) $l)
@@ -321,8 +268,10 @@ where
       | (_, #[]) => go irs' (patAcc.push hole) propAcc
       | (#[patArg], props) => go irs' (patAcc.push lbi) <| propAcc.push <| ←
           ``(∀ $patArg ∈ $l, $(← foldlAnd props))
-      | (patArgs, props) => go irs' (patAcc.push lbi) <| propAcc.push <| ←
-          ``(∀ $l'bi ∈ $l, let $(← foldrProd <| ← toTerms patArgs):term := $l'; $(← foldlAnd props))
+      | (patArgs, props) =>
+        let prod ← liftMacroM <| foldrProd <| ← toTerms patArgs
+        go irs' (patAcc.push lbi) <| propAcc.push <| ←
+          ``(∀ $l'bi ∈ $l, let $prod:term := $l'; $(← foldlAnd props))
     | .optional ir, .optional pir => do
       if ir.size != pir.size then
         throwErrorAt prodIdent "length of child optional ({ir.size}) doesn't match length of parent optional ({pir.size})"
@@ -336,8 +285,10 @@ where
       | (_, #[]) => go irs' (patAcc.push hole) propAcc
       | (#[patArg], props) => go irs' (patAcc.push lbi) <| propAcc.push <| ←
           ``(∀ $patArg:binderIdent ∈ $l, $(← foldlAnd props))
-      | (patArgs, props) => go irs' (patAcc.push lbi) <| propAcc.push <| ←
-          ``(∀ $l'bi ∈ $l, let $(← foldrProd <| ← toTerms patArgs):term := $l'; $(← foldlAnd props))
+      | (patArgs, props) =>
+        let prod ← liftMacroM <| foldrProd <| ← toTerms patArgs
+        go irs' (patAcc.push lbi) <| propAcc.push <| ←
+          ``(∀ $l'bi ∈ $l, let $prod:term := $l'; $(← foldlAnd props))
     | _, _ => throwErrorAt prodIdent "mismatched syntax"
 
 private
@@ -348,9 +299,9 @@ def freeName (varName : Name) (typeName : Name) : CommandElabM Name := do
   | .str .anonymous s => return typeName ++ Name.appendAfter `free s |>.appendAfter "s"
   | n => return typeName ++ `free ++ n.appendAfter "s"
 
-partial
+private partial
 def toFreeMatchAlt (prodId : Ident) (ir : Array IR) (subst : Name × Name)
-  (binders : Array Name) : CommandElabM (TSyntax `Lean.Parser.Term.matchAltExpr) := do
+  (binders : Array Name) : CommandElabM (TSyntax ``Lean.Parser.Term.matchAltExpr) := do
   let (patArgs, appendArgs) ← goMany ir
   let rhs ← foldlAppend appendArgs
   `(matchAltExpr| | $prodId $patArgs* => $rhs)
@@ -378,18 +329,20 @@ where
       | (#[], _) => return (none, none)
       | (_, #[]) => return (← ``(_), none)
       | (patArgs, appendArgs) =>
+        let prod ← liftMacroM <| foldrProd patArgs
         return (
           l,
-          ← `((List.mapMem $l fun $(← foldrProd patArgs) _ => $(← foldlAppend appendArgs)).flatten)
+          ← `((List.mapMem $l fun $prod _ => $(← foldlAppend appendArgs)).flatten)
         )
     | .optional ir => match ← goMany ir with
       | (#[], _) => return (none, none)
       | (_, #[]) => return (← ``(_), none)
       | (patArgs, appendArgs) =>
+        let prod ← liftMacroM <| foldrProd patArgs
         return (
           l,
           ← `(
-            (Option.mapMem $l fun $(← foldrProd patArgs) _ => $(← foldlAppend appendArgs)).getD []
+            (Option.mapMem $l fun $prod _ => $(← foldlAppend appendArgs)).getD []
           )
         )
 
@@ -407,10 +360,10 @@ def containsVar (varName : Name) (ir : Array IR) (ids binders : Array Name) : Bo
     | mk _ (.sepBy ir _)
     | mk _ (.optional ir) => containsVar varName ir ids binders
 
-partial
+private partial
 def toLocallyClosedCtors (prodId locallyClosedId idxId : Ident) (qualified : Name) (ir : Array IR)
   (subst : Name × Name) (ids binders : Array Name)
-  : CommandElabM (Array (TSyntax `Lean.Parser.Command.ctor)) := do
+  : CommandElabM (Array (TSyntax ``Lean.Parser.Command.ctor)) := do
   if containsVar subst.fst ir ids binders then
     let #[mk _ (.category _)] := ir |
       throwErrorAt prodId "generation of locally closed definitions is not yet supported for complicated productions"
@@ -434,8 +387,8 @@ where
   inc := ir.any fun
     | mk l (.category n) => n == subst.fst && binders.contains l.getId
     | _ => false
-  go (irs : Array IR) (patAcc : TSyntaxArray `Lean.binderIdent := #[]) (propAcc : Array Term := #[])
-    : CommandElabM (TSyntaxArray `Lean.binderIdent × Array Term) := do
+  go (irs : Array IR) (patAcc : TSyntaxArray ``Lean.binderIdent := #[]) (propAcc : Array Term := #[])
+    : CommandElabM (TSyntaxArray ``Lean.binderIdent × Array Term) := do
     let some (mk l ir) := irs[0]? | return (patAcc, propAcc)
     let irs := irs.extract 1 irs.size
 
@@ -473,14 +426,14 @@ where
           `(∀ $patArg:binderIdent ∈ $l, $(← foldlAnd props))
       | (patArgs, props) =>
         let propAcc' ← props.mapM fun prop =>
-          do `(∀ x ∈ $l, let $(← foldrProd <| ← toTerms patArgs):term := x; $prop)
+          do `(∀ x ∈ $l, let $(← liftMacroM <| foldrProd <| ← toTerms patArgs):term := x; $prop)
         go irs (patAcc.push lbi) <| propAcc ++ propAcc'
 
-
+private
 def substName (varName : Name) : CommandElabM Name :=
   return varName.replacePrefix (← getCurrNamespace) .anonymous |>.appendAfter "_subst"
 
-partial
+private partial
 def toSubstPatternAndArgs (ir : Array IR) (varType valType : Name) (varId valId :  Ident)
   (bindOf? binderId? : Option Ident) : CommandElabM (Option (Array Term × Array Term)) := do
   let patsAndArgsAndFounds ← ir.filterMapM fun (mk l irt) => do
@@ -499,12 +452,16 @@ def toSubstPatternAndArgs (ir : Array IR) (varType valType : Name) (varId valId 
       let some (pattern, args) ←
         toSubstPatternAndArgs ir varType valType varId valId bindOf? binderId? |
         return some (l, (l : Term), false)
-      return some (l, ← `(List.mapMem $l fun $(← foldrProd pattern) _ => $(← foldrProd args)), true)
+      let patProd ← liftMacroM <| foldrProd pattern
+      let argsProd ← liftMacroM <| foldrProd args
+      return some (l, ← `(List.mapMem $l fun $patProd _ => $argsProd), true)
     | .optional ir =>
       let some (pattern, args) ←
         toSubstPatternAndArgs ir varType valType varId valId bindOf? binderId? |
         return some (l, (l : Term), false)
-      let arg ← `(Option.mapMem $l fun $(← foldrProd pattern) _ => $(← foldrProd args))
+      let patProd ← liftMacroM <| foldrProd pattern
+      let argsProd ← liftMacroM <| foldrProd args
+      let arg ← `(Option.mapMem $l fun $patProd _ => $argsProd)
       return some (l, arg, true)
   let (pats, argsAndFounds) := patsAndArgsAndFounds.unzip
   let (args, founds) := argsAndFounds.unzip
@@ -513,10 +470,11 @@ def toSubstPatternAndArgs (ir : Array IR) (varType valType : Name) (varId valId 
   else
     return none
 
+private
 def openName (varName : Name) : CommandElabM Name :=
   return varName.replacePrefix (← getCurrNamespace) .anonymous |>.appendAfter "_open"
 
-partial
+private partial
 def toVarOpenPatternAndArgs (ir : Array IR) (varType valType : Name) (varId idxId :  Ident)
   (bindOf? binderId? : Option Ident) : CommandElabM (Option (Array Term × Array Term)) := do
   let patsAndArgsAndFounds ← ir.filterMapM fun (mk l irt) => do
@@ -537,12 +495,16 @@ def toVarOpenPatternAndArgs (ir : Array IR) (varType valType : Name) (varId idxI
       let some (pattern, args) ←
         toVarOpenPatternAndArgs ir varType valType varId idxId bindOf? binderId? |
         return some (l, (l : Term), false)
-      return some (l, ← `(List.mapMem $l fun $(← foldrProd pattern) _ => $(← foldrProd args)), true)
+      let patProd ← liftMacroM <| foldrProd pattern
+      let argsProd ← liftMacroM <| foldrProd args
+      return some (l, ← `(List.mapMem $l fun $patProd _ => $argsProd), true)
     | .optional ir =>
       let some (pattern, args) ←
         toVarOpenPatternAndArgs ir varType valType varId idxId bindOf? binderId? |
         return some (l, (l : Term), false)
-      let arg ← `(Option.mapMem $l fun $(← foldrProd pattern) _ => $(← foldrProd args))
+      let patProd ← liftMacroM <| foldrProd pattern
+      let argsProd ← liftMacroM <| foldrProd args
+      let arg ← `(Option.mapMem $l fun $patProd _ => $argsProd)
       return some (l, arg, true)
   let (pats, argsAndFounds) := patsAndArgsAndFounds.unzip
   let (args, founds) := argsAndFounds.unzip
@@ -551,7 +513,7 @@ def toVarOpenPatternAndArgs (ir : Array IR) (varType valType : Name) (varId idxI
   else
     return none
 
-partial
+private partial
 def toValOpenPatternAndArgs (ir : Array IR) (varType valType : Name) (valId idxId :  Ident)
   (bindOf? binderId? : Option Ident) : CommandElabM (Option (Array Term × Array Term)) := do
   let patsAndArgsAndFounds ← ir.filterMapM fun (mk l irt) => do
@@ -569,12 +531,16 @@ def toValOpenPatternAndArgs (ir : Array IR) (varType valType : Name) (valId idxI
       let some (pattern, args) ←
         toValOpenPatternAndArgs ir varType valType valId idxId bindOf? binderId? |
         return some (l, (l : Term), false)
-      return some (l, ← `(List.mapMem $l fun $(← foldrProd pattern) _ => $(← foldrProd args)), true)
+      let patProd ← liftMacroM <| foldrProd pattern
+      let argsProd ← liftMacroM <| foldrProd args
+      return some (l, ← `(List.mapMem $l fun $patProd _ => $argsProd), true)
     | .optional ir =>
       let some (pattern, args) ←
         toValOpenPatternAndArgs ir varType valType valId idxId bindOf? binderId? |
         return some (l, (l : Term), false)
-      let arg ← `(Option.mapMem $l fun $(← foldrProd pattern) _ => $(← foldrProd args))
+      let patProd ← liftMacroM <| foldrProd pattern
+      let argsProd ← liftMacroM <| foldrProd args
+      let arg ← `(Option.mapMem $l fun $patProd _ => $argsProd)
       return some (l, arg, true)
   let (pats, argsAndFounds) := patsAndArgsAndFounds.unzip
   let (args, founds) := argsAndFounds.unzip
@@ -583,10 +549,11 @@ def toValOpenPatternAndArgs (ir : Array IR) (varType valType : Name) (valId idxI
   else
     return none
 
+private
 def closeName (varName : Name) : CommandElabM Name :=
   return varName.replacePrefix (← getCurrNamespace) .anonymous |>.appendAfter "_close"
 
-partial
+private partial
 def toClosePatternAndArgs (ir : Array IR) (varType valType : Name) (varId idxId :  Ident)
   (bindOf? binderId? : Option Ident) : CommandElabM (Option (Array Term × Array Term)) := do
   let patsAndArgsAndFounds ← ir.filterMapM fun (mk l irt) => do
@@ -607,12 +574,16 @@ def toClosePatternAndArgs (ir : Array IR) (varType valType : Name) (varId idxId 
       let some (pattern, args) ←
         toClosePatternAndArgs ir varType valType varId idxId bindOf? binderId? |
         return some (l, (l : Term), false)
-      return some (l, ← `(List.mapMem $l fun $(← foldrProd pattern) _ => $(← foldrProd args)), true)
+      let patProd ← liftMacroM <| foldrProd pattern
+      let argsProd ← liftMacroM <| foldrProd args
+      return some (l, ← `(List.mapMem $l fun $patProd _ => $argsProd), true)
     | .optional ir =>
       let some (pattern, args) ←
         toClosePatternAndArgs ir varType valType varId idxId bindOf? binderId? |
         return some (l, (l : Term), false)
-      let arg ← `(Option.mapMem $l fun $(← foldrProd pattern) _ => $(← foldrProd args))
+      let patProd ← liftMacroM <| foldrProd pattern
+      let argsProd ← liftMacroM <| foldrProd args
+      let arg ← `(Option.mapMem $l fun $patProd _ => $argsProd)
       return some (l, arg, true)
   let (pats, argsAndFounds) := patsAndArgsAndFounds.unzip
   let (args, founds) := argsAndFounds.unzip
@@ -621,7 +592,43 @@ def toClosePatternAndArgs (ir : Array IR) (varType valType : Name) (varId idxId 
   else
     return none
 
+def symbolEmbedIdent := mkIdent ``Lott.symbolEmbed
+
 /- Metavariable syntax. -/
+
+@[macro Lott.symbolEmbed]
+private
+def identImpl : Macro := fun stx => do
+  let Syntax.node _ ``Lott.symbolEmbed #[
+    .atom _ "[[",
+    .node _ _ #[ident@(Lean.Syntax.ident ..)],
+    .atom _ "]]"
+  ] := stx | Macro.throwUnsupported
+  return ident
+
+@[macro symbolEmbed]
+private
+def appImpl : Macro := fun stx => do
+  let Syntax.node _ ``Lott.symbolEmbed #[
+    .atom _ "[[",
+    .node _ _ #[«fun», .atom _ "@", idx],
+    .atom _ "]]"
+  ] := stx | Macro.throwUnsupported
+  `(([[$(.mk «fun»):Lott.Symbol]] : _ → _) $(.mk idx):term)
+
+@[macro symbolEmbed]
+private
+def boundImpl : Macro := fun stx => do
+  let Lean.Syntax.node _ ``Lott.symbolEmbed #[
+    Lean.Syntax.atom _ "[[",
+    Lean.Syntax.node _ _ #[
+      Lean.Syntax.ident ..,
+      Lean.Syntax.atom _ "$",
+      num@(Lean.Syntax.node _ `num _)
+    ],
+    Lean.Syntax.atom _ "]]"
+  ] := stx | Macro.throwUnsupported
+  `(.bound $(.mk num))
 
 elab_rules : command | `($[locally_nameless%$ln]? metavar $names,*) => do
   let names := names.getElems.toList
@@ -677,78 +684,49 @@ elab_rules : command | `($[locally_nameless%$ln]? metavar $names,*) => do
     let aliasName@(.str .anonymous nameStr) := alias.getId | throwUnsupportedSyntax
     let parserIdent := mkIdentFrom alias <| canon.getId ++ aliasName.appendAfter "_parser"
     elabCommand <| ←
-      `(@[$(mkIdent parserAttrName):ident] def $parserIdent : Parser :=
+      `(@[Lott.Symbol_parser, $(mkIdent parserAttrName):ident]
+        private
+        def $parserIdent : Parser :=
           leadingNode $(quote catName) Parser.maxPrec <| Lott.identPrefix $(quote nameStr))
-    let parserIdent := mkIdentFrom alias <| canon.getId ++ aliasName.appendAfter "_idx_parser"
-    elabCommand <| ←
-      `(@[$(mkIdent parserAttrName):ident] def $parserIdent : TrailingParser :=
-          trailingNode $(quote catName) Parser.maxPrec 0 <|
-            checkNoWsBefore >> "@" >> checkLineEq >> (Parser.ident <|> Parser.numLit))
+
     if locallyNameless then
       let parserIdent := mkIdentFrom alias <| canon.getId ++ aliasName.appendAfter "_bound_parser"
       elabCommand <| ←
-        `(@[$(mkIdent parserAttrName):ident] def $parserIdent : Parser :=
+        `(@[Lott.Symbol_parser, $(mkIdent parserAttrName):ident]
+          private
+          def $parserIdent : Parser :=
             leadingNode $(quote catName) Parser.maxPrec <|
               Lott.identPrefix $(quote nameStr) >> "$" >> num)
 
-  -- Define elaboration.
-  let catIdent := mkIdent catName
-  let termElabName := mkIdentFrom canon <| canon.getId.appendAfter "TermElab"
-  let (rhs, bound) ← if locallyNameless then
-      pure (
-        ← `(do
-          if isBinder then
-              let type ← Lean.Elab.Term.elabType <| mkIdent $(quote <| canonQualified.appendAfter "Id")
-              Lean.Elab.Term.elabTerm ident type
-            else
-              let type ← Lean.Elab.Term.elabType <| mkIdent $(quote canonQualified)
-              let expr ← Lean.Elab.Term.elabTerm (Syntax.mkCApp `Coe.coe #[.mk ident]) type
-              Meta.liftMetaM <| Meta.reduce expr),
-        #[← `(matchAltExpr|
-              | isBinder, Lean.Syntax.node _ $(quote catName) #[
-                  ident@(Lean.Syntax.ident ..),
-                  Lean.Syntax.atom _ "$",
-                  num@(Lean.Syntax.node _ `num _)
-                ] => do
-                if isBinder then
-                  throwUnsupportedSyntax
-                else
-                  let num ← Lean.Elab.Term.elabNumLit num <| some (.const `Nat [])
-                  return (Lean.Expr.const $(quote <| canonQualified ++ `bound) []).app num)]
-      )
-    else
-      pure (← `(do
-          let type ← Lean.Elab.Term.elabType <| mkIdent $(quote canonQualified)
-          Lean.Elab.Term.elabTerm ident type), #[])
+  let parserIdent := mkIdentFrom canon <| canon.getId.appendAfter "_idx_parser"
   elabCommand <| ←
-    `(@[lott_term_elab $catIdent] def $termElabName : Lott.Elab.TermElab
-        | isBinder, Lean.Syntax.node _ $(quote catName) #[ident@(Lean.Syntax.ident ..)] => $rhs
-        | isBinder, Lean.Syntax.node _ $(quote catName) #[
-            Lean.Syntax.node _ $(quote catName) #[fun'@(Lean.Syntax.ident ..)],
-            Lean.Syntax.atom _ "@",
-            idx
-          ] => do
-          let typeName := if isBinder then
-              $(quote <| canonQualified.appendAfter "Id")
-            else
-              $(quote canonQualified)
-          let type ← Lean.Elab.Term.elabType <| mkIdent typeName
-          let natType := Expr.const `Nat []
-          let funType := Expr.forallE `x natType type .default
-          let funExpr ← Lean.Elab.Term.elabTerm fun' funType
-          let idxExpr ← Lean.Elab.Term.elabTerm idx natType
-          return Expr.app funExpr idxExpr
-        $bound:matchAlt*
-        | _, stx => no_error_if_unused% Lean.Elab.throwUnsupportedSyntax)
+    `(@[Lott.Symbol_parser, $(mkIdent parserAttrName):ident]
+      private
+      def $parserIdent : TrailingParser :=
+        trailingNode $(quote catName) Parser.maxPrec 0 <|
+          checkNoWsBefore >> "@" >> checkLineEq >> (Parser.ident <|> Parser.numLit))
 
 /- Non-terminal syntax. -/
 
+@[macro symbolEmbed]
 private
-inductive ProductionType where
-  | normal
-  | sugar (desugar' : Term)
-  | customElab (elab' : Term)
-deriving BEq
+def variableImpl : Macro := fun stx => do
+  let Syntax.node _ ``Lott.symbolEmbed #[
+    .atom _ "[[",
+    .node _ _ #[.node _ _ #[ident@(Lean.Syntax.ident ..)] ],
+    .atom _ "]]"
+  ] := stx | Macro.throwUnsupported
+  return ident
+
+@[macro symbolEmbed]
+private
+def varAppImpl : Macro := fun stx => do
+  let Syntax.node _ ``Lott.symbolEmbed #[
+    .atom _ "[[",
+    .node info kind #[.node _ _ #[«fun», .atom _ "@", idx] ],
+    .atom _ "]]"
+  ] := stx | Macro.throwUnsupported
+  `(($(Syntax.mkSymbolEmbed (.node info kind #[«fun»])) : _ → _) $(.mk idx))
 
 private
 structure BindConfig where
@@ -770,7 +748,7 @@ private
 structure Production where
   name : Ident
   ir : Array IR
-  type : ProductionType
+  expand? : Option Term
   bindConfig? : Option BindConfig
   ids : Array Name
 
@@ -784,7 +762,7 @@ structure NonTerminal where
   aliases : Array Ident
   prods : Array Production
   parent? : Option Ident
-  substitutions : Option (Array (Name × Name))
+  substitutions? : Option (Array (Name × Name))
 
 namespace NonTerminal
 
@@ -857,9 +835,9 @@ def elabNonTerminals (nts : Array Syntax) : CommandElabM Unit := do
     for name in names do
       setEnv <| aliasExt.addEntry (← getEnv) { canon, alias := ns ++ name.getId }
 
-    if let some parent' := parent? then
-      let parent' ← resolveSymbol parent' (allowSuffix := false)
-      setEnv <| childExt.addEntry (← getEnv) { canon, parent' }
+    if let some parent := parent? then
+      let parent ← resolveSymbol parent (allowSuffix := false)
+      setEnv <| childExt.addEntry (← getEnv) { canon, parent }
 
   -- Transform syntax into non-terminal structure.
   let nts ← nts.mapM fun nt => do
@@ -869,7 +847,7 @@ def elabNonTerminals (nts : Array Syntax) : CommandElabM Unit := do
     let aliases := names.extract 1 names.size
 
     let prodAndSubsts ← prods.mapM fun prod => do
-      let `(Production| | $[$ps]* : $name $[nosubst%$ns?]? $[$bindConfig?]? $[(id $ids?,*)]? $[(desugar := $desugar?)]? $[(elab := $elab?)]?) := prod
+      let `(Production| | $[$ps]* : $name $[nosubst%$ns?]? $[$bindConfig?]? $[(id $ids?,*)]? $[(expand := $expand?)]?) := prod
         | throwUnsupportedSyntax
       let ids := ids?.getD (.mk #[]) |>.getElems
 
@@ -897,55 +875,49 @@ def elabNonTerminals (nts : Array Syntax) : CommandElabM Unit := do
             logWarningAt name "name not found in syntax"
         return res
 
-      let type ← match desugar?, elab? with
-      | some _, some _ => throwUnsupportedSyntax
-      | some desugar, none => pure <| .sugar desugar
-      | none, some elab' => pure <| .customElab elab'
-      | none, _ => pure <| .normal
-
-      return ({ name, ir, type, bindConfig?, ids := ids.map TSyntax.getId }, subst)
+      return ({ name, ir, expand?, bindConfig?, ids := ids.map TSyntax.getId }, subst)
 
     let (prods, substs) := prodAndSubsts.unzip
     let qualified := (← getCurrNamespace) ++ canon.getId
-    let substitutions := if parent?.isSome || ns.isSome then
+    let substitutions? := if parent?.isSome || ns.isSome then
         none
       else
         substs.filterMap id |>.map ((·, qualified))
 
-    let parent? ← parent?.mapM fun parent' =>
-      return mkIdentFrom parent' <| ← resolveSymbol parent' (allowSuffix := false)
+    let parent? ← parent?.mapM fun parent =>
+      return mkIdentFrom parent <| ← resolveSymbol parent (allowSuffix := false)
 
-    return { canon, aliases, prods, parent?, substitutions : NonTerminal }
+    return { canon, aliases, prods, parent?, substitutions? : NonTerminal }
 
   -- Define mutual inductives and parser categories.
   let defsAndInductives ← nts.mapM fun nt@{ canon, prods, parent?, .. } => do
     setEnv <| ← registerParserCategory (← getEnv) (← nt.parserAttrName) (← nt.catName) .symbol
     setEnv <| ← registerParserCategory (← getEnv) (← nt.varParserAttrName) (← nt.varCatName) .symbol
 
-    let some parent' := parent? |
-      let ctors ← prods.filterMapM fun prod@{ name, ir, type, ids, .. } => do
-        let .normal := type | return none
+    let some parent := parent? |
+      let ctors ← prods.filterMapM fun prod@{ name, ir, expand?, ids, .. } => do
+        let none := expand? | return none
         let ctorType ← IR.toTypeArrSeq ir canon ids prod.binders
         `(ctor| | $name:ident : $ctorType)
       let inductive' ← `(inductive $canon where $ctors*)
       return (none, inductive')
-    let some { normalProds, .. } := symbolExt.getState (← getEnv) |>.find? parent'.getId
-      | throwErrorAt parent' "unknown parent {parent'.getId}"
+    let some { normalProds, .. } := symbolExt.getState (← getEnv) |>.find? parent.getId
+      | throwErrorAt parent "unknown parent {parent.getId}"
 
-    let isIdent := mkIdentFrom canon <| parent'.getId ++ canon.getId.appendBefore "Is"
-    let ctors ← prods.mapM fun prod@{ name, ir, type, .. } => match type with
-      | .sugar ref | .customElab ref =>
-        throwErrorAt ref "nonterminal with parent can only contain normal productions"
-      | .normal => do
+    let isIdent := mkIdentFrom canon <| parent.getId ++ canon.getId.appendBefore "Is"
+    let ctors ← prods.mapM fun prod@{ name, ir, expand?, .. } => match expand? with
+      | some ref =>
+        throwErrorAt ref "nonterminal with parent cannot contain productions with expand specifier"
+      | none => do
         let some pir := normalProds.find? name.getId
           | throwErrorAt name "normal production with matching name not found in parent"
 
-        IR.toIsChildCtor name isIdent (← nt.qualified) parent'.getId ir pir prod.binders
+        IR.toIsChildCtor name isIdent (← nt.qualified) parent.getId ir pir prod.binders
     let inductive' ←
-      `(inductive $(mkIdentFrom isIdent <| `_root_ ++ isIdent.getId) : $parent' → Prop where
+      `(inductive $(mkIdentFrom isIdent <| `_root_ ++ isIdent.getId) : $parent → Prop where
           $ctors*)
 
-    return (some <| ← `(def $canon := { x : $parent' // $isIdent x }), inductive')
+    return (some <| ← `(def $canon := { x : $parent // $isIdent x }), inductive')
   let (defs, inductives) := defsAndInductives.unzip
   elabMutualCommands inductives
   elabMutualCommands <| defs.filterMap id
@@ -953,33 +925,33 @@ def elabNonTerminals (nts : Array Syntax) : CommandElabM Unit := do
   let ntsMap ← nts.foldlM (init := mkNameMap _) fun acc nt => return acc.insert (← nt.qualified) nt
   let namePairCmp | (a₁, a₂), (b₁, b₂) => Name.quickCmp a₁ b₁ |>.«then» <| Name.quickCmp a₂ b₂
   let nts ← nts.mapM fun nt => do
-    if nt.substitutions.isNone then
+    if nt.substitutions?.isNone then
       return nt
 
     let mut substitutions' := RBTree.empty (cmp := namePairCmp)
     for n in ← nt.shallowClosure ntsMap do
       let substitutions? ← match ntsMap.find? n with
-        | some { substitutions, .. } => pure substitutions
+        | some { substitutions?, .. } => pure substitutions?
         | none =>
           let some { substitutions, .. } := symbolExt.getState (← getEnv) |>.find? n | continue
           pure substitutions
       let some substitutions := substitutions? | continue
       for subst in substitutions do
         substitutions' := substitutions'.insert subst
-    return { nt with substitutions := substitutions'.toArray : NonTerminal }
+    return { nt with substitutions? := substitutions'.toArray : NonTerminal }
 
-  for nt@{ canon, aliases, prods, parent?, substitutions } in nts do
+  for nt@{ canon, aliases, prods, parent?, substitutions? } in nts do
     -- Add symbol to environment extension before proceeding so that lookups of things within the
     -- current mutual still work properly.
-    let normalProds := prods.foldl (init := mkNameMap _) fun acc { name, ir, type, .. } =>
-      if let .normal := type then acc.insert name.getId ir else acc
+    let normalProds := prods.foldl (init := mkNameMap _) fun acc { name, ir, expand?, .. } =>
+      if expand?.isNone then acc.insert name.getId ir else acc
     setEnv <| symbolExt.addEntry (← getEnv)
-      { qualified := ← nt.qualified, normalProds, substitutions := substitutions.getD #[] }
+      { qualified := ← nt.qualified, normalProds, substitutions := substitutions?.getD #[] }
 
   let isLocallyNameless (varName : Name) : CommandElabM Bool :=
     return metaVarExt.getState (← getEnv) |>.find! varName
 
-  for nt@{ canon, aliases, prods, parent?, substitutions } in nts do
+  for nt@{ canon, aliases, prods, parent?, substitutions? } in nts do
     -- Define production and substitution parsers.
     let canonName := canon.getId
     let attrIdent := mkIdent <| ← nt.parserAttrName
@@ -987,12 +959,18 @@ def elabNonTerminals (nts : Array Syntax) : CommandElabM Unit := do
       for { name, ir, .. } in prods do
         let (val, type) ← IR.toParser ir nt.canon.getId symbolPrefix
         let parserIdent := mkIdentFrom name <| canonName ++ name.getId |>.appendAfter "_parser"
-        elabCommand <| ← `(@[Lott.Symbol_parser, $attrIdent:ident] def $parserIdent : $type := $val)
+        elabCommand <| ←
+          `(@[Lott.Symbol_parser, $attrIdent:ident]
+            private
+            def $parserIdent : $type := $val)
 
-    for (varName, valName) in substitutions.getD #[] do
+    let substitutions := substitutions?.getD #[]
+    for (varName, valName) in substitutions do
       let parserIdent := mkIdent <| canonName ++ varName |>.appendAfter "_subst_parser"
       elabCommand <| ←
-        `(@[Lott.Symbol_parser, $attrIdent:ident] def $parserIdent : TrailingParser :=
+        `(@[Lott.Symbol_parser, $attrIdent:ident]
+          private
+          def $parserIdent : TrailingParser :=
             trailingNode $(quote <| ← nt.catName) Parser.maxPrec 0 <|
               "[" >> categoryParser $(quote <| symbolPrefix ++ valName) 0 >> " / " >>
                 categoryParser $(quote <| symbolPrefix ++ varName) 0 >> "]")
@@ -1003,25 +981,31 @@ def elabNonTerminals (nts : Array Syntax) : CommandElabM Unit := do
 
       let parserIdent := mkIdent <| canonName ++ varName |>.appendAfter "_open_parser"
       elabCommand <| ←
-        `(@[Lott.Symbol_parser, $attrIdent:ident] def $parserIdent : TrailingParser :=
+        `(@[Lott.Symbol_parser, $attrIdent:ident]
+          private
+          def $parserIdent : TrailingParser :=
             trailingNode $(quote <| ← nt.catName) Parser.maxPrec 0 <|
               checkNoWsBefore >> "^" >> categoryParser $(quote <| symbolPrefix ++ varName) 0 >>
-              Parser.optional (checkNoWsBefore >> "#" >> checkLineEq >> Parser.numLit))
+                Parser.optional (checkNoWsBefore >> "#" >> checkLineEq >> Parser.numLit))
 
       let parserIdent := mkIdent <| canonName ++ valName |>.appendAfter "_open_parser"
       elabCommand <| ←
-        `(@[Lott.Symbol_parser, $attrIdent:ident] def $parserIdent : TrailingParser :=
+        `(@[Lott.Symbol_parser, $attrIdent:ident]
+          private
+          def $parserIdent : TrailingParser :=
             trailingNode $(quote <| ← nt.catName) Parser.maxPrec 0 <|
               checkNoWsBefore >> "^^" >> categoryParser $(quote <| symbolPrefix ++ valName) 0 >>
-              Parser.optional (checkNoWsBefore >> "#" >> checkLineEq >> Parser.numLit))
+                Parser.optional (checkNoWsBefore >> "#" >> checkLineEq >> Parser.numLit))
 
       let parserIdent := mkIdent <| canonName ++ varName |>.appendAfter "_close_parser"
       elabCommand <| ←
-        `(@[Lott.Symbol_parser, $attrIdent:ident] def $parserIdent : Parser :=
+        `(@[Lott.Symbol_parser, $attrIdent:ident]
+          private
+          def $parserIdent : Parser :=
             leadingNode $(quote <| ← nt.catName) Parser.maxPrec <|
               "\\" >> categoryParser $(quote <| symbolPrefix ++ varName) 0 >>
-              Parser.optional (checkNoWsBefore >> "#" >> checkLineEq >> Parser.numLit) >>
-              "^" >> categoryParser $(quote <| ← nt.catName) 0)
+                Parser.optional (checkNoWsBefore >> "#" >> checkLineEq >> Parser.numLit) >>
+                "^" >> categoryParser $(quote <| ← nt.catName) 0)
 
     -- Define variable parsers, plus variable category parser in symbol category.
     let varAttrIdent := mkIdent <| ← nt.varParserAttrName
@@ -1029,183 +1013,183 @@ def elabNonTerminals (nts : Array Syntax) : CommandElabM Unit := do
       let aliasName@(.str .anonymous nameStr) := alias.getId | throwUnsupportedSyntax
       let parserIdent := mkIdentFrom alias <| canonName ++ aliasName.appendAfter "_parser"
       elabCommand <| ←
-        `(@[$varAttrIdent:ident] def $parserIdent : Parser :=
+        `(@[$varAttrIdent:ident]
+          private
+          def $parserIdent : Parser :=
             leadingNode $(quote <| ← nt.varCatName) Parser.maxPrec <|
               Lott.identPrefix $(quote nameStr))
 
-    -- TODO: Should this have `Lott.Symbol_parser`?
+    let parserIdent := mkIdentFrom canon <| canon.getId.appendAfter "_idx_parser"
+    elabCommand <| ←
+      `(@[$varAttrIdent:ident]
+        private
+        def $parserIdent : TrailingParser :=
+          trailingNode $(quote <| ← nt.varCatName) Parser.maxPrec 0 <|
+            checkNoWsBefore >> "@" >> checkLineEq >> (Parser.ident <|> Parser.numLit))
+
     let varParserIdent := mkIdentFrom canon <| canonName.appendAfter "_variable_parser"
     elabCommand <| ←
-      `(@[$attrIdent:ident] def $varParserIdent : Parser :=
+      `(@[Lott.Symbol_parser, $attrIdent:ident]
+        private
+        def $varParserIdent : Parser :=
           leadingNode $(quote <| ← nt.catName) Parser.maxPrec <|
-            categoryParser $(quote <| ← nt.varCatName) Parser.maxPrec >>
-            Parser.optional
-              (checkNoWsBefore >> "@" >> checkLineEq >> (Parser.ident <|> Parser.numLit)))
+            categoryParser $(quote <| ← nt.varCatName) Parser.maxPrec)
 
     -- Define parser in parent.
-    if let some parent' := parent? then
-      let parentQualified := parent'.getId
+    if let some parent := parent? then
+      let parentQualified := parent.getId
       let parentParserCatName := symbolPrefix ++ parentQualified
       let parentParserAttrName := parentParserCatName.appendAfter "_parser"
       let parentParserIdent :=
-        mkIdentFrom parent' <| `_root_ ++ parentQualified ++ canonName.appendAfter "_parser"
+        mkIdentFrom parent <| `_root_ ++ parentQualified ++ canonName.appendAfter "_parser"
       elabCommand <| ←
-        `(@[$(mkIdent parentParserAttrName):ident] def $parentParserIdent : Parser :=
+        `(@[Lott.Symbol_parser, $(mkIdent parentParserAttrName):ident]
+          private
+          def $parentParserIdent : Parser :=
             leadingNode $(quote parentParserCatName) Parser.maxPrec <|
               categoryParser $(quote <| ← nt.catName) 0)
 
-    -- Define desugar macros and elaboration.
-    let catIdent := mkIdent <| ← nt.catName
-    let termProdMatchAlts ← if parent?.isSome then pure #[] else
-      prods.filterMapM fun prod@{ name, ir, type, ids, .. } => do
-        let patternArgs ← IR.toPatternArgs ir
-
-        if let .sugar desugar' := type then
-          let macroIdent := mkIdentFrom name <| canonName ++ name.getId |>.appendAfter "_macro"
-          elabCommand <| ←
-            `(@[macro $catIdent] def $macroIdent : Lean.Macro
-                | Lean.Syntax.node _ $(quote <| ← nt.catName) #[$patternArgs,*] => $desugar'
-                | _ => Lean.Macro.throwUnsupported)
-          return none
-
-        let seqItems ← IR.toTermSeqItems ir canon.getId ids prod.binders
+    -- Define macros.
+    let catName ← nt.catName
+    let catIdent := mkIdent catName
+    for prod@{ name, ir, expand?, ids, .. } in prods do
+      let patternArgs ← IR.toPatternArgs ir
+      let seqItems ← IR.toTermSeqItems ir canon.getId ids prod.binders
+      let rest ← expand?.getDM do
         let exprArgs ← IR.toExprArgs ir ids prod.binders
-        let rest ← if let .customElab elab' := type then
-            pure elab'
-          else
-            `(term| return Lean.mkAppN
-                      (Lean.Expr.const $(quote <| ns ++ canonName ++ name.getId) [])
-                      #[$exprArgs,*])
+        `(return Syntax.mkCApp $(quote <| ns ++ canonName ++ name.getId) #[$exprArgs,*])
 
-        `(matchAltExpr|
-          | _, Lean.Syntax.node _ $(quote <| ← nt.catName) #[$patternArgs,*] => do
+      let macroName := mkIdentFrom name <| canonName ++ name.getId |>.appendAfter "Impl"
+      elabCommand <| ←
+        `(@[macro $symbolEmbedIdent]
+          private
+          def $macroName : Macro := fun stx => do
+            let Lean.Syntax.node _ ``Lott.symbolEmbed #[
+              Lean.Syntax.atom _ "[[",
+              Lean.Syntax.node _ $(quote catName) #[$patternArgs,*],
+              Lean.Syntax.atom _ "]]"
+            ] := stx | Macro.throwUnsupported
             $seqItems*
             $rest:term)
 
-    let termSubstMatchAlts ← if parent?.isSome then pure #[] else
-      substitutions.getD #[] |>.mapM fun (varName, valName) => do
-        let substName := ns ++ canonName ++ (← substName varName)
-        `(matchAltExpr|
-            | _, Lean.Syntax.node _ $(quote <| ← nt.catName) #[
-                base@(Lean.Syntax.node _ $(quote <| ← nt.catName) _),
+    -- TODO: Figure out how normal open and close should work when a varName appears more than once.
+    for (varName, valName) in substitutions do
+      let substName := ns ++ canonName ++ (← substName varName)
+      let macroName :=
+        mkIdentFrom canon <| canonName ++ varName ++ `Subst ++ valName |>.appendAfter "Impl"
+      elabCommand <| ←
+        `(@[macro $symbolEmbedIdent]
+          private
+          def $macroName : Macro := fun stx => do
+            let Lean.Syntax.node _ ``Lott.symbolEmbed #[
+              Lean.Syntax.atom _ "[[",
+              Lean.Syntax.node _ $(quote catName) #[
+                base@(Lean.Syntax.node _ $(quote catName) _),
                 Lean.Syntax.atom _ "[",
                 val@(Lean.Syntax.node _ $(quote <| symbolPrefix ++ valName) _),
                 Lean.Syntax.atom _ "/",
                 var@(Lean.Syntax.node _ $(quote <| symbolPrefix ++ varName) _),
                 Lean.Syntax.atom _ "]"
-              ] => do
-              let baseExpr ← Lott.Elab.elabTerm $(quote <| symbolPrefix ++ ns ++ canonName) false base
-              let varExpr ← Lott.Elab.elabTerm $(quote <| symbolPrefix ++ varName) true var
-              let valExpr ← Lott.Elab.elabTerm $(quote <| symbolPrefix ++ valName) false val
-              return Lean.mkApp3 (Expr.const $(quote substName) []) baseExpr varExpr valExpr)
+              ],
+              Lean.Syntax.atom _ "]]"
+            ] := stx | Macro.throwUnsupported
+            return Syntax.mkCApp $(quote substName) #[
+              Lott.Syntax.mkSymbolEmbed base,
+              Lott.Syntax.mkSymbolEmbed var,
+              Lott.Syntax.mkSymbolEmbed val
+            ])
 
-    let termOpenMatchAlts ← if parent?.isSome then pure #[] else
-      substitutions.getD #[] |>.filterMapM fun (varName, _) => do
-        if !(← isLocallyNameless varName) then return none
+      if !(← isLocallyNameless varName) then
+        continue
 
-        let openName := ns ++ canonName ++ (← openName varName)
-        return some <| ←
-          `(matchAltExpr|
-            | _, Lean.Syntax.node _ $(quote <| ← nt.catName) #[
-                base@(Lean.Syntax.node _ $(quote <| ← nt.catName) _),
+      let macroName := mkIdentFrom canon <| canonName ++ varName ++ `Open |>.appendAfter "Impl"
+      let varOpenName := ns ++ canonName ++ (← openName varName)
+      elabCommand <| ←
+        `(@[macro $symbolEmbedIdent]
+          private
+          def $macroName : Macro := fun stx => do
+            let Lean.Syntax.node _ ``Lott.symbolEmbed #[
+              Lean.Syntax.atom _ "[[",
+              Lean.Syntax.node _ $(quote catName) #[
+                base@(Lean.Syntax.node _ $(quote catName) _),
                 Lean.Syntax.atom _ "^",
                 var@(Lean.Syntax.node _ $(quote <| symbolPrefix ++ varName) _),
                 Lean.Syntax.node _ `null level
-              ] => do
-              let baseExpr ← Lott.Elab.elabTerm $(quote <| symbolPrefix ++ ns ++ canonName) false base
-              let varExpr ← Lott.Elab.elabTerm $(quote <| symbolPrefix ++ varName) true var
-              let natType := Expr.const `Nat []
-              let lvlExpr? ← level[1]?.mapM fun lvl => Lean.Elab.Term.elabTerm lvl natType
-              return Lean.mkApp3 (Expr.const $(quote openName) []) baseExpr varExpr <|
-                lvlExpr?.getD <| Expr.lit <| Literal.natVal 0)
+              ],
+              Lean.Syntax.atom _ "]]"
+            ] := stx | Macro.throwUnsupported
+            return Syntax.mkCApp $(quote varOpenName) <| #[
+              Lott.Syntax.mkSymbolEmbed base,
+              Lott.Syntax.mkSymbolEmbed var
+            ] ++ (level[1]?.map TSyntax.mk).toArray)
 
-    let termOpen'MatchAlts ← if parent?.isSome then pure #[] else
-      substitutions.getD #[] |>.filterMapM fun (varName, valName) => do
-        if !(← isLocallyNameless varName) then return none
-
-        let openName := ns ++ canonName ++ (← openName valName)
-        return some <| ←
-          `(matchAltExpr|
-            | _, Lean.Syntax.node _ $(quote <| ← nt.catName) #[
-                base@(Lean.Syntax.node _ $(quote <| ← nt.catName) _),
+      let macroName := mkIdentFrom canon <| canonName ++ valName ++ `Open |>.appendAfter "Impl"
+      let valOpenName := ns ++ canonName ++ (← openName valName)
+      elabCommand <| ←
+        `(@[macro $symbolEmbedIdent]
+          private
+          def $macroName : Macro := fun stx => do
+            let Lean.Syntax.node _ ``Lott.symbolEmbed #[
+              Lean.Syntax.atom _ "[[",
+              Lean.Syntax.node _ $(quote catName) #[
+                base@(Lean.Syntax.node _ $(quote catName) _),
                 Lean.Syntax.atom _ "^^",
                 val@(Lean.Syntax.node _ $(quote <| symbolPrefix ++ valName) _),
                 Lean.Syntax.node _ `null level
-              ] => do
-              let baseExpr ← Lott.Elab.elabTerm $(quote <| symbolPrefix ++ ns ++ canonName) false base
-              let valExpr ← Lott.Elab.elabTerm $(quote <| symbolPrefix ++ valName) false val
-              let natType := Expr.const `Nat []
-              let lvlExpr? ← level[1]?.mapM fun lvl => Lean.Elab.Term.elabTerm lvl natType
-              return Lean.mkApp3 (Expr.const $(quote openName) []) baseExpr valExpr <|
-                lvlExpr?.getD <| Expr.lit <| Literal.natVal 0)
+              ],
+              Lean.Syntax.atom _ "]]"
+            ] := stx | Macro.throwUnsupported
+            return Syntax.mkCApp $(quote valOpenName) <| #[
+              Lott.Syntax.mkSymbolEmbed base,
+              Lott.Syntax.mkSymbolEmbed val
+            ] ++ (level[1]?.map TSyntax.mk).toArray)
 
-    let termCloseMatchAlts ← if parent?.isSome then pure #[] else
-      substitutions.getD #[] |>.filterMapM fun (varName, _) => do
-        if !(← isLocallyNameless varName) then return none
-
-        let closeName := ns ++ canonName ++ (← closeName varName)
-        return some <| ←
-          `(matchAltExpr|
-            | _, Lean.Syntax.node _ $(quote <| ← nt.catName) #[
+      let macroName := mkIdentFrom canon <| canonName ++ varName ++ `Close |>.appendAfter "Impl"
+      let closeName := ns ++ canonName ++ (← closeName varName)
+      elabCommand <| ←
+        `(@[macro $symbolEmbedIdent]
+          private
+          def $macroName : Macro := fun stx => do
+            let Lean.Syntax.node _ ``Lott.symbolEmbed #[
+              Lean.Syntax.atom _ "[[",
+              Lean.Syntax.node _ $(quote catName) #[
                 Lean.Syntax.atom _ "\\",
                 var@(Lean.Syntax.node _ $(quote <| symbolPrefix ++ varName) _),
                 Lean.Syntax.node _ `null level,
                 Lean.Syntax.atom _ "^",
-                base@(Lean.Syntax.node _ $(quote <| ← nt.catName) _)
-              ] => do
-              let varExpr ← Lott.Elab.elabTerm $(quote <| symbolPrefix ++ varName) true var
-              let baseExpr ← Lott.Elab.elabTerm $(quote <| symbolPrefix ++ ns ++ canonName) false base
-              let natType := Expr.const `Nat []
-              let lvlExpr? ← level[1]?.mapM fun lvl => Lean.Elab.Term.elabTerm lvl natType
-              return Lean.mkApp3 (Expr.const $(quote closeName) []) baseExpr varExpr <|
-                lvlExpr?.getD <| Expr.lit <| Literal.natVal 0)
+                base@(Lean.Syntax.node _ $(quote catName) _)
+              ],
+              Lean.Syntax.atom _ "]]"
+            ] := stx | Macro.throwUnsupported
+            return Syntax.mkCApp $(quote closeName) <| #[
+              Lott.Syntax.mkSymbolEmbed base,
+              Lott.Syntax.mkSymbolEmbed var
+            ] ++ (level[1]?.map TSyntax.mk).toArray)
 
-    let termElabIdent := mkIdentFrom canon <| canonName.appendAfter "TermElab"
-    elabCommand <| ←
-      `(@[lott_term_elab $catIdent] def $termElabIdent : Lott.Elab.TermElab
-          $termProdMatchAlts:matchAlt*
-          $termSubstMatchAlts:matchAlt*
-          $termOpenMatchAlts:matchAlt*
-          $termOpen'MatchAlts:matchAlt*
-          $termCloseMatchAlts:matchAlt*
-          | _, Lean.Syntax.node _ $(quote <| ← nt.catName) #[
-              Lean.Syntax.node _ $(quote <| ← nt.varCatName) #[ident@(Lean.Syntax.ident ..)],
-              Lean.Syntax.node _ `null #[]
-            ] => do
-            let type ← Lean.Elab.Term.elabType <| mkIdent $(quote <| ns ++ canonName)
-            Lean.Elab.Term.elabTerm ident type
-          | _, Lean.Syntax.node _ $(quote <| ← nt.catName) #[
-              Lean.Syntax.node _ $(quote <| ← nt.varCatName) #[fun'@(Lean.Syntax.ident ..)],
-              Lean.Syntax.node _ `null #[Lean.Syntax.atom _ "@", idx]
-            ] => do
-            let type ← Lean.Elab.Term.elabType <| mkIdent $(quote <| ns ++ canonName)
-            let natType := Expr.const `Nat []
-            let funType := Expr.forallE `x natType type .default
-            let funExpr ← Lean.Elab.Term.elabTerm fun' funType
-            let idxExpr ← Lean.Elab.Term.elabTerm idx natType
-            return Expr.app funExpr idxExpr
-          | _, _ => no_error_if_unused% Lean.Elab.throwUnsupportedSyntax)
-
-    if let some parent' := parent? then
+    if let some parent := parent? then
       let qualified ← nt.qualified
-      let catName ← nt.catName
-      let parentQualified := parent'.getId
-      let parentCatName := symbolPrefix ++ parentQualified
+      let parentCatName := symbolPrefix ++ parent.getId
       let parentCatIdent := mkIdent parentCatName
-      let parentTermElabName :=
-        mkIdent <| `_root_ ++ parentQualified ++ canon.getId.appendAfter "TermElab"
+      let parentMacroName :=
+        mkIdent <| `_root_ ++ parent.getId ++ canon.getId.appendAfter "Impl"
       elabCommand <| ←
-        `(@[lott_term_elab $parentCatIdent] def $parentTermElabName : Lott.Elab.TermElab
-            | _, Lean.Syntax.node _ $(quote parentCatName) #[
-                stx@(Lean.Syntax.node _ $(quote <| ← nt.catName) _)
-              ] => do
-              let type ← Lean.Elab.Term.elabType <| mkIdent $(quote qualified)
-              let e ← Lott.Elab.elabTerm $(quote catName) false stx
-              return Lean.Expr.proj `Subtype 0 e
-            | _, _ => no_error_if_unused% Lean.Elab.throwUnsupportedSyntax)
+        `(@[macro $symbolEmbedIdent]
+          private
+          def $parentMacroName : Macro := fun stx => do
+            let Lean.Syntax.node _ ``Lott.symbolEmbed #[
+              Lean.Syntax.atom _ "[[",
+              Lean.Syntax.node _ $(quote parentCatName) #[
+                stx@(Lean.Syntax.node _ $(quote catName) _)
+              ],
+              Lean.Syntax.atom _ "]]"
+            ] := stx | Macro.throwUnsupported
+            return Lean.Syntax.mkCApp ``Subtype.val #[
+              Lean.Syntax.mkTypeAscription (Lott.Syntax.mkSymbolEmbed stx) <|
+                Lean.mkIdent $(quote qualified)
+            ])
 
   -- Add metavar functions.
-  let allSubstitutions := nts.map fun { substitutions, .. } => substitutions.getD #[]
+  let allSubstitutions := nts.map (·.substitutions?.getD #[])
   let uniqueSubstitutions :=
     allSubstitutions.flatten.foldl Std.HashSet.insert Std.HashSet.empty |>.toArray
   for subst@(varTypeName, valTypeName) in uniqueSubstitutions do
@@ -1220,12 +1204,12 @@ def elabNonTerminals (nts : Array Syntax) : CommandElabM Unit := do
     let varId ← mkFreshIdent varTypeId
     let valId ← mkFreshIdent valTypeId
 
-    let substDefs ← nts.filterMapM fun nt@{ canon, aliases, prods, parent?, substitutions } => do
-      if !(substitutions.getD #[]).contains subst then
+    let substDefs ← nts.filterMapM fun nt@{ canon, aliases, prods, parent?, substitutions? } => do
+      if !(substitutions?.getD #[]).contains subst then
         return none
 
-      let matchAlts ← prods.filterMapM fun { name, ir, type, bindConfig?, .. } => do
-        let .normal := type | return none
+      let matchAlts ← prods.filterMapM fun { name, ir, expand?, bindConfig?, .. } => do
+        let none := expand? | return none
         let prodId := mkIdent <| canon.getId ++ name.getId
 
         let bindOf? := bindConfig?.map fun { of, .. } => of
@@ -1265,12 +1249,12 @@ def elabNonTerminals (nts : Array Syntax) : CommandElabM Unit := do
 
     let idxId ← mkFreshIdent varTypeId
 
-    let varOpenDefs ← nts.filterMapM fun nt@{ canon, aliases, prods, parent?, substitutions } => do
-      if !(substitutions.getD #[]).contains subst then
+    let varOpenDefs ← nts.filterMapM fun nt@{ canon, aliases, prods, parent?, substitutions? } => do
+      if !(substitutions?.getD #[]).contains subst then
         return none
 
-      let matchAlts ← prods.filterMapM fun { name, ir, type, bindConfig?, .. } => do
-        let .normal := type | return none
+      let matchAlts ← prods.filterMapM fun { name, ir, expand?, bindConfig?, .. } => do
+        let none := expand? | return none
         let prodId := mkIdent <| canon.getId ++ name.getId
 
         let bindOf? := bindConfig?.map fun { of, .. } => of
@@ -1304,12 +1288,12 @@ def elabNonTerminals (nts : Array Syntax) : CommandElabM Unit := do
 
     elabMutualCommands varOpenDefs
 
-    let valOpenDefs ← nts.filterMapM fun nt@{ canon, aliases, prods, parent?, substitutions } => do
-      if !(substitutions.getD #[]).contains subst then
+    let valOpenDefs ← nts.filterMapM fun nt@{ canon, aliases, prods, parent?, substitutions? } => do
+      if !(substitutions?.getD #[]).contains subst then
         return none
 
-      let matchAlts ← prods.filterMapM fun { name, ir, type, bindConfig?, .. } => do
-        let .normal := type | return none
+      let matchAlts ← prods.filterMapM fun { name, ir, expand?, bindConfig?, .. } => do
+        let none := expand? | return none
         let prodId := mkIdent <| canon.getId ++ name.getId
 
         let bindOf? := bindConfig?.map fun { of, .. } => of
@@ -1347,12 +1331,12 @@ def elabNonTerminals (nts : Array Syntax) : CommandElabM Unit := do
 
     elabMutualCommands valOpenDefs
 
-    let closeDefs ← nts.filterMapM fun nt@{ canon, aliases, prods, parent?, substitutions } => do
-      if !(substitutions.getD #[]).contains subst then
+    let closeDefs ← nts.filterMapM fun nt@{ canon, aliases, prods, parent?, substitutions? } => do
+      if !(substitutions?.getD #[]).contains subst then
         return none
 
-      let matchAlts ← prods.filterMapM fun { name, ir, type, bindConfig?, .. } => do
-        let .normal := type | return none
+      let matchAlts ← prods.filterMapM fun { name, ir, expand?, bindConfig?, .. } => do
+        let none := expand? | return none
         let prodId := mkIdent <| canon.getId ++ name.getId
 
         let bindOf? := bindConfig?.map fun { of, .. } => of
@@ -1387,13 +1371,13 @@ def elabNonTerminals (nts : Array Syntax) : CommandElabM Unit := do
     elabMutualCommands closeDefs
 
     let freeDefs ←
-      nts.filterMapM fun nt@{ canon, aliases, prods, parent?, substitutions } => do
-        if !(substitutions.getD #[]).contains subst then
+      nts.filterMapM fun nt@{ canon, aliases, prods, parent?, substitutions? } => do
+        if !(substitutions?.getD #[]).contains subst then
           return none
 
         let freeId := mkIdent <| ← freeName varTypeName <| ← nt.qualified
-        let matchAlts ← prods.filterMapM fun prod@{ name, ir, type, .. } => do
-          let .normal := type | return none
+        let matchAlts ← prods.filterMapM fun prod@{ name, ir, expand?, .. } => do
+          let none := expand? | return none
           let prodId := mkIdentFrom name <| (← nt.qualified) ++ name.getId
           toFreeMatchAlt prodId ir subst prod.binders
         return some <| ← `(def $freeId : $canon → List $varTypeId $matchAlts:matchAlt*)
@@ -1401,13 +1385,13 @@ def elabNonTerminals (nts : Array Syntax) : CommandElabM Unit := do
     elabMutualCommands freeDefs
 
     let locallyClosedInductives ←
-      nts.filterMapM fun nt@{ canon, aliases, prods, parent?, substitutions } => do
-        if !(substitutions.getD #[]).contains subst then
+      nts.filterMapM fun nt@{ canon, aliases, prods, parent?, substitutions? } => do
+        if !(substitutions?.getD #[]).contains subst then
           return none
 
         let locallyClosedId := mkIdent <| ← locallyClosedName varTypeName <| ← nt.qualified
-        let ctors ← prods.mapM fun prod@{ name, ir, type, ids, .. } => do
-          let .normal := type | return #[]
+        let ctors ← prods.mapM fun prod@{ name, ir, expand?, ids, .. } => do
+          let none := expand? | return #[]
           toLocallyClosedCtors name locallyClosedId idxId (← nt.qualified) ir subst ids prod.binders
         return some <| ←
           `(inductive $locallyClosedId : $canon → (optParam Nat 0) → Prop where $ctors.flatten*)
@@ -1438,23 +1422,27 @@ elab_rules : command | `(judgement_syntax $[$ps]* : $name $[(id $ids?,*)]?) => d
   if type != (← `(term| Parser)) then throwError "invalid left recursive judgement syntax"
   let parserIdent := mkIdentFrom name <| name.getId.appendAfter "_parser"
   elabCommand <| ←
-    `(@[Lott.Judgement_parser, $(mkIdent parserAttrName):ident] def $parserIdent : Parser := $val)
+    `(@[Lott.Judgement_parser, $(mkIdent parserAttrName):ident]
+      private
+      def $parserIdent : Parser := $val)
 
-  -- Define elaboration.
+  -- Define macro.
   let patternArgs ← IR.toPatternArgs ir
   let termSeqItems ← IR.toTermSeqItems ir name.getId ids #[]
   let exprArgs ← IR.toExprArgs ir ids #[]
   let catIdent := mkIdent catName
-  let termElabIdent := mkIdentFrom name <| name.getId.appendAfter "TermElab"
+  let macroName := mkIdentFrom name <| name.getId.appendAfter "Impl"
   elabCommand <| ←
-    `(@[lott_term_elab $catIdent] def $termElabIdent : Lott.Elab.TermElab
-        | _, Lean.Syntax.node _ $(quote catName) #[$patternArgs,*] => do
-          $termSeqItems*
-          let name := $(quote qualified)
-          let some e ← Lean.Elab.Term.resolveId? <| Lean.mkIdent name
-            | Lean.throwError s!"failed to resolve judgement identifier {name} (potential use of judgement embedding before judgement declaration)"
-          return Lean.mkAppN e #[$exprArgs,*]
-        | _, _ => no_error_if_unused% Lean.Elab.throwUnsupportedSyntax)
+    `(@[macro $(mkIdent `Lott.judgementEmbed)]
+      private
+      def $macroName : Macro := fun stx => do
+        let Lean.Syntax.node _ ``Lott.judgementEmbed #[
+          Lean.Syntax.atom _ "[[",
+          Lean.Syntax.node _ $(quote catName) #[$patternArgs,*],
+          Lean.Syntax.atom _ "]]"
+        ] := stx | Macro.throwUnsupported
+        $termSeqItems*
+        return Syntax.mkApp (mkIdent $(quote qualified)) #[$exprArgs,*])
 
 private
 def elabJudgementDecls (jds : Array Syntax) : CommandElabM Unit := do
@@ -1473,7 +1461,10 @@ def elabJudgementDecls (jds : Array Syntax) : CommandElabM Unit := do
       let conclusionKind := conclusion.raw.getKind
       let expectedKind := judgementPrefix ++ catName
       if conclusionKind != expectedKind then
-        throwErrorAt conclusion "found conclusion judgement syntax kind{indentD conclusionKind}\nexpected to find kind{indentD expectedKind}\nall conclusions of inference rules in a judgement declaration must be the judgement which is being defined"
+        throwErrorAt conclusion
+          "found conclusion judgement syntax kind{indentD conclusionKind}\
+          expected to find kind{indentD expectedKind}\
+          all conclusions of inference rules in a judgement declaration must be the judgement which is being defined"
       let ctorType ← jms.foldrM (init := ← `(term| [[$conclusion:Lott.Judgement]]))
         fun «judgement» acc => `([[$«judgement»:Lott.Judgement]] → $acc)
       `(ctor| | $name:ident $binders* : $ctorType)
@@ -1484,4 +1475,31 @@ elab_rules : command
   | `($jd:Lott.JudgementDecl) => elabJudgementDecls #[jd]
   | `(mutual $[$jds:Lott.JudgementDecl]* end) => elabJudgementDecls jds
 
-end Lott.Elab
+/- Term embedding syntax. -/
+
+/-
+You can't put a hole inside an embedding to ignore something, so it's generally desirable to not be
+bugged about embedding pattern variables being unused.
+-/
+register_option linter.unusedVariables.lottSymbolEmbeddingPatternVars : Bool := {
+  defValue := false
+  descr :=
+    "enable the 'unused variables' linter to mark unused lott symbol embedding pattern variables"
+}
+
+def getLinterUnusedVariablesLottSymbolEmbeddingPatternVars (o : Options) : Bool :=
+  o.get linter.unusedVariables.lottSymbolEmbeddingPatternVars.name
+    (Lean.Linter.getLinterUnusedVariables o &&
+      linter.unusedVariables.lottSymbolEmbeddingPatternVars.defValue)
+
+@[unused_variables_ignore_fn]
+private
+def symbolEmbeddingPatternVars : Lean.Linter.IgnoreFunction := fun _ stack opts =>
+  !getLinterUnusedVariablesLottSymbolEmbeddingPatternVars opts && (
+    let stackBeforeMatchAlt := stack.takeWhile fun (stx, _) =>
+      !stx.isOfKind ``Lean.Parser.Term.matchAlt
+    stackBeforeMatchAlt.length != stack.length &&
+      stackBeforeMatchAlt.any fun (stx, _) => stx.isOfKind ``Lott.symbolEmbed
+  )
+
+end Lott
