Lott/Elab/Nat.lean
@@ -1,6 +1,6 @@
 import Lott.Elab
 
-namespace Lott.Elab
+namespace Lott
 
 open Lean
 open Lean.Elab
@@ -11,21 +11,36 @@ declare_syntax_cat Lott.Symbol.Nat
 run_cmd setEnv <| aliasExt.addEntry (← getEnv) { canon := `Nat, alias := `n }
 
 @[Lott.Symbol.Nat_parser]
+private
 def nat.n_parser : Parser := leadingNode `Lott.Symbol.Nat maxPrec <| identPrefix "n"
 
 @[Lott.Symbol.Nat_parser]
+private
 def nat.num_parser : Parser := leadingNode `Lott.Symbol.Nat maxPrec numLit
 
 @[Lott.Symbol.Nat_parser]
+private
 def nat.term_parser : Parser :=
   leadingNode `Lott.Symbol.Nat maxPrec <| "(" >> checkLineEq >> termParser >> checkLineEq >> ")"
 
-@[lott_term_elab Lott.Symbol.Nat]
-def natTermElab : TermElab
-  | _, .node _ `Lott.Symbol.Nat #[n@(.ident ..)]
-  | _, .node _ `Lott.Symbol.Nat #[n@(.node _ `num _)]
-  | _, .node _ `Lott.Symbol.Nat #[.atom _ "(", n, .atom _ ")"] =>
-    Term.elabTerm n <| .some (.const `Nat [])
-  | _, _ => throwUnsupportedSyntax
+@[macro symbolEmbed]
+private
+def natImpl : Macro
+  | .node _ `Lott.symbolEmbed #[
+      .atom _ "[[",
+      .node _ `Lott.Symbol.Nat #[n@(.ident ..)],
+      .atom _ "]]"
+    ]
+  | .node _ `Lott.symbolEmbed #[
+      .atom _ "[[",
+      .node _ `Lott.Symbol.Nat #[n@(.node _ `num _)],
+      .atom _ "]]"
+    ]
+  | .node _ `Lott.symbolEmbed #[
+      .atom _ "[[",
+      .node _ `Lott.Symbol.Nat #[.atom _ "(", n, .atom _ ")"],
+      .atom _ "]]"
+    ] => return n
+  | _ => Macro.throwUnsupported
 
-end Lott.Elab
+end Lott
