Lott/Parser.lean
@@ -1,3 +1,4 @@
+import Lean.Elab
 import Lean.Parser
 
 namespace Lott
@@ -8,32 +9,30 @@ open Lean.Parser.Syntax
 
 /- Common trailing syntax. -/
 
-declare_syntax_cat Lott.Trailing
-
-def isPrefixOf (prefix' : String) (n : Name) : Bool := prefix'.isPrefixOf n.getRoot.getString!
-
-def identPrefixFn (prefix' : String) : ParserFn := fun c s =>
+private
+def identPrefixFn («prefix» : String) : ParserFn := fun c s =>
   let s := tokenFn ["identifier"] c s
   if s.hasError then
     s
   else
     match s.stxStack.back with
     | .ident _ _ val _ =>
-      if !isPrefixOf prefix' val then
-        s.mkUnexpectedTokenError s!"identifier beginning with '{prefix'}'"
+      if !prefix.isPrefixOf val.getRoot.getString! then
+        s.mkUnexpectedTokenError s!"identifier beginning with '{«prefix»}'"
       else
         s
     | _ => s.mkUnexpectedTokenError "identifier"
 
-def identPrefix (prefix' : String) : Parser := {
-  fn := identPrefixFn prefix'
+def identPrefix («prefix» : String) : Parser where
+  fn := identPrefixFn «prefix»
   info := mkAtomicInfo "ident"
-}
 
-@[combinator_parenthesizer identPrefix] def identPrefix.parenthesizer (_prefix : String) :=
+@[combinator_parenthesizer identPrefix]
+def identPrefix.parenthesizer (_ : String) :=
   PrettyPrinter.Parenthesizer.visitToken
 
-@[combinator_formatter identPrefix] def identPrefix.formatter (_parser : String) :=
+@[combinator_formatter identPrefix]
+def identPrefix.formatter (_ : String) :=
   PrettyPrinter.Formatter.rawIdentNoAntiquot.formatter
 
 /- Metavariable syntax. -/
@@ -45,8 +44,7 @@ syntax "locally_nameless"? "metavar " ident,+ : command
 declare_syntax_cat Lott.Symbol
 declare_syntax_cat Lott.BindConfig
 declare_syntax_cat Lott.IdConfig
-declare_syntax_cat Lott.DesugarConfig
-declare_syntax_cat Lott.ElabConfig
+declare_syntax_cat Lott.ExpandConfig
 declare_syntax_cat Lott.Production
 declare_syntax_cat Lott.NonTerminal
 
@@ -61,18 +59,19 @@ def id := nonReservedSymbol "id"
 syntax "(" id ident,+ ")" : Lott.IdConfig
 
 private
-def desugar := nonReservedSymbol "desugar"
+def expand := nonReservedSymbol "expand"
 
-syntax "(" desugar " := " term ")" : Lott.DesugarConfig
-
-syntax "(" "elab" " := " term ")" : Lott.ElabConfig
+syntax "(" expand " := " term ")" : Lott.ExpandConfig
 
 def prodArg  := leading_parser
   Parser.optional (atomic (ident >> checkNoWsBefore "no space before ':'" >> ":")) >> syntaxParser argPrec
 
-syntax " | " prodArg+ " : " withPosition(ident (lineEq "nosubst")?) atomic(Lott.BindConfig)? atomic(Lott.IdConfig)? atomic(Lott.DesugarConfig)? (Lott.ElabConfig)? : Lott.Production
+syntax " | " prodArg+ " : " withPosition(ident (lineEq "nosubst")?) atomic(Lott.BindConfig)? atomic(Lott.IdConfig)? (Lott.ExpandConfig)? : Lott.Production
 
-syntax "nosubst"? "nonterminal " ("(" "parent" " := " ident ")")? ident,+ " := " Lott.Production* : Lott.NonTerminal
+private
+def parent := nonReservedSymbol "parent"
+
+syntax "nosubst"? "nonterminal " ("(" parent " := " ident ")")? ident,+ " := " Lott.Production* : Lott.NonTerminal
 
 syntax Lott.NonTerminal : command
 
@@ -95,8 +94,14 @@ syntax Lott.JudgementDecl : command
 
 /- Term embedding syntax. -/
 
--- Mostly copied from Lean/Parser/Extension.lean, Lean/PrettyPrinter/Formatter.lean, and
--- Lean/PrettyPrinter/Parenthesizer.lean, but with a prefix automatically added to the name.
+syntax (name := symbolEmbed) "[[" withPosition(Lott.Symbol) "]]" : term
+
+syntax (name := judgementEmbed) "[[" withPosition(Lott.Judgement) "]]" : term
+
+/-
+Like Lean/Parser/Extension.lean, Lean/PrettyPrinter/Formatter.lean, and
+Lean/PrettyPrinter/Parenthesizer.lean, but with the Lott.Symbol prefix automatically added.
+-/
 private
 def parserOfStackFn (offset : Nat) : ParserFn := fun c s => Id.run do
   let stack := s.stxStack
@@ -138,10 +143,6 @@ def parserOfStack.parenthesizer (offset : Nat) (_prec : Nat := 0) : Parenthesize
 private
 def lottSymbolParser := incQuotDepth (parserOfStack 1)
 
-syntax (name := lott_symbol_embed) "[[" ident "|" lottSymbolParser "]]" : term
-
-syntax "[[" withPosition(Lott.Symbol) "]]" : term
-
-syntax "[[" withPosition(Lott.Judgement) "]]" : term
+macro "[[" ident "|" symbol:lottSymbolParser "]]" : term => `([[$(.mk symbol.raw):Lott.Symbol]])
 
 end Lott
